@prefix owl: <http://www.w3.org/2002/07/owl#> .
@prefix rdf: <http://www.w3.org/1999/02/22-rdf-syntax-ns#> .
@prefix xsd: <http://www.w3.org/2001/XMLSchema#> .
@prefix ocp: <http://www.semanticweb.org/albrechtvaatz/ontologies/2025/3/OCP#> .
@prefix rdfs: <http://www.w3.org/2000/01/rdf-schema#> .

<http://www.semanticweb.org/albrechtvaatz/ontologies/2022/9/cMod_V0.1> rdf:type owl:Ontology ;
                                                                        owl:imports <http://www.w3.org/2006/time#> ;
                                                                        rdfs:comment "Ontology for Chronological Processes (OCP) is an extension of the OWL-Time ontology, designed to better describe unfinished, iterative, and ongoing processes."@en .

#################################################################
#    Object Properties
#################################################################


	###  http://www.semanticweb.org/albrechtvaatz/ontologies/2025/3/OCP#beginsAfter
	ocp:beginsAfter rdf:type owl:ObjectProperty ;
		rdfs:subPropertyOf <http://www.w3.org/2006/time#hasBeginning> ;
		rdfs:domain <http://www.w3.org/2006/time#Interval> ;
		rdfs:range <http://www.w3.org/2006/time#TemporalEntity> ;
		owl:inverseOf ocp:beginsBefore ;
		rdf:type owl:TransitiveProperty ;
		rdfs:comment "This property represents the chronological order of beginnings between two temporal entities, used to indicate that T1’s beginning occurs after T2’s beginning, without defining the order of their ends."@en ;
		rdfs:label "begins after"@en .


	###  http://www.semanticweb.org/albrechtvaatz/ontologies/2025/3/OCP#beginsBefore
	ocp:beginsBefore rdf:type owl:ObjectProperty ;
		rdfs:subPropertyOf <http://www.w3.org/2006/time#hasBeginning> ;
		rdfs:domain <http://www.w3.org/2006/time#Interval> ;
		rdfs:range <http://www.w3.org/2006/time#TemporalEntity> ;
		owl:inverseOf ocp:beginsAfter ;
		rdf:type owl:TransitiveProperty ;
		rdfs:comment "This property represents the chronological order of beginnings between two temporal entities, used to indicate that T1’s beginning occurs before T2’s beginning, without defining the order of their ends."@en ;
		rdfs:label "begins before"@en .


	###  http://www.semanticweb.org/albrechtvaatz/ontologies/2025/3/OCP#beginsWith
	ocp:beginsWith rdf:type owl:ObjectProperty ;
		rdfs:subPropertyOf <http://www.w3.org/2006/time#hasBeginning> ;
		rdfs:domain <http://www.w3.org/2006/time#Interval> ;
		rdfs:range <http://www.w3.org/2006/time#TemporalEntity> ;
		rdfs:comment "This property represents the chronological order of beginnings between two temporal entities, used to indicate that T1’s beginning occurs on the same day as T2’s beginning, without defining the order of their ends."@en ;
		rdfs:label "begins with"@en .


    ###  http://www.semanticweb.org/albrechtvaatz/ontologies/2025/3/OCP#belongsToCycle
    ocp:belongsToCycle rdf:type owl:ObjectProperty ;
		rdfs:domain <http://www.w3.org/2006/time#Instant> ;
		rdfs:range ocp:Cycle ;
		rdfs:comment "This property represents the connection between a time:Instant and a cycle."@en ;
		rdfs:label "belongs to cycle"@en .				


    ###  http://www.semanticweb.org/albrechtvaatz/ontologies/2025/3/OCP#belongsToInstant
    ocp:belongsToInstant rdf:type owl:ObjectProperty ;
		rdfs:domain ocp:Phase ;
		rdfs:range <http://www.w3.org/2006/time#Instant> ;
		owl:inverseOf ocp:belongsToPhase ;
		rdfs:comment "This property represents the link of a ocp:Phase to a time:Instant."@en ;
		rdfs:label "belongs to instant"@en .


    ###  http://www.semanticweb.org/albrechtvaatz/ontologies/2025/3/OCP#belongsToProcess
    ocp:belongsToProcess a rdf:Property ;
        rdfs:domain <http://www.w3.org/2006/time#TemporalEntity> ;
		rdfs:range ocp:Process ;
		rdfs:comment "This property represents the embedding of a time:Entity within a ocp:Process."@en ;
        rdfs:label "belongs to Process" .


    ###  http://www.semanticweb.org/albrechtvaatz/ontologies/2025/3/OCP#belongsToPhase
    ocp:belongsToPhase rdf:type owl:ObjectProperty ;
		rdfs:domain <http://www.w3.org/2006/time#Instant> ;
		rdfs:range ocp:Phase ;
		owl:inverseOf ocp:belongsToInstant ;
		rdfs:comment "This property represents the connection between a time:Instant and a ocp:Phase."@en ;
		rdfs:label "belongs to phase"@en .


	###  http://www.semanticweb.org/albrechtvaatz/ontologies/2025/3/OCP#endsAfter
	ocp:endsAfter rdf:type owl:ObjectProperty ;
		rdfs:subPropertyOf <http://www.w3.org/2006/time#hasEnd> ;
		rdfs:domain <http://www.w3.org/2006/time#Interval> ;
		rdfs:range <http://www.w3.org/2006/time#TemporalEntity> ;
		owl:inverseOf ocp:endsBefore ;
		rdf:type owl:TransitiveProperty ;
		rdfs:comment "This property represents the chronological order of endings between two temporal entities, used to indicate that T1’s end occurs after T2’s end, without defining the order of their beginnings."@en ;
		rdfs:label "ends after"@en .


	###  http://www.semanticweb.org/albrechtvaatz/ontologies/2025/3/OCP#endsBefore
	ocp:endsBefore rdf:type owl:ObjectProperty ;
		rdfs:subPropertyOf <http://www.w3.org/2006/time#hasEnd> ;
		rdfs:domain <http://www.w3.org/2006/time#Interval> ;
		rdfs:range <http://www.w3.org/2006/time#TemporalEntity> ;
		owl:inverseOf ocp:endsAfter ;
		rdf:type owl:TransitiveProperty ;
		rdfs:comment "This property represents the chronological order of endings between two temporal entities, used to indicate that T1’s end occurs before T2’s end, without defining the order of their beginnings."@en ;
		rdfs:label "ends before"@en .


	###  http://www.semanticweb.org/albrechtvaatz/ontologies/2025/3/OCP#endsCycle
	ocp:endsCycle rdf:type owl:ObjectProperty ;
		rdfs:subPropertyOf <http://www.w3.org/2006/time#hasEnd> ;
		rdfs:domain <http://www.w3.org/2006/time#Instant> ;
		rdfs:range ocp:Cycle ;
		rdfs:comment "This property represents the relationship between an instant and a cycle, used to mark instants that end an ongoing cycle within a phase."@en ;
		rdfs:label "ends cycle"@en .


	###  http://www.semanticweb.org/albrechtvaatz/ontologies/2025/3/OCP#endsPhase
	ocp:endsPhase rdf:type owl:ObjectProperty ;
		rdfs:subPropertyOf <http://www.w3.org/2006/time#hasEnd> ;
		rdfs:domain <http://www.w3.org/2006/time#Instant> ;
		rdfs:range ocp:Phase ;
		rdfs:comment "This property represents the relationship between an instant and a phase, used to mark instants that end an ongoing phase."@en ;
		rdfs:label "ends phase"@en .


	###  http://www.semanticweb.org/albrechtvaatz/ontologies/2025/3/OCP#endsWith
	ocp:endsWith rdf:type owl:ObjectProperty ;
		rdfs:subPropertyOf <http://www.w3.org/2006/time#hasEnd> ;
		rdfs:domain <http://www.w3.org/2006/time#Interval> ;
		rdfs:range <http://www.w3.org/2006/time#TemporalEntity> ;
		rdfs:comment "This property represents the chronological order of endings between two temporal entities, used to indicate that T1’s end occurs on the same day as T2’s end, without defining the order of their beginnings."@en ;
		rdfs:label "ends with"@en .


	###  http://www.semanticweb.org/albrechtvaatz/ontologies/2025/3/OCP#hasActualBeginning
	ocp:hasActualBeginning rdf:type owl:ObjectProperty ;
		rdfs:subPropertyOf <http://www.w3.org/2006/time#hasBeginning> ;
		rdfs:domain <http://www.w3.org/2006/time#Interval> ;
		rdfs:range <http://www.w3.org/2006/time#Instant> ;
		rdfs:comment "This property represents the connection between an interval and an instant, used to mark the actual beginning of a phase."@en ;
		rdfs:label "has actual beginning"@en .


    ###  http://www.semanticweb.org/albrechtvaatz/ontologies/2025/3/OCP#hasActualEnd
    ocp:hasActualEnd rdf:type owl:ObjectProperty ;
		rdfs:subPropertyOf <http://www.w3.org/2006/time#hasEnd> ;
		rdfs:domain <http://www.w3.org/2006/time#Interval> ;
		rdfs:range  <http://www.w3.org/2006/time#Instant> ;
		rdfs:comment "This property represents the connection between an interval and an instant, used to mark the actual end of a phase."@en ;
		rdfs:label "has actual end"@en .


    ###  http://www.semanticweb.org/albrechtvaatz/ontologies/2025/3/OCP#hasEstimatedBeginning
    ocp:hasEstimatedBeginning rdf:type owl:ObjectProperty ;
		rdfs:subPropertyOf <http://www.w3.org/2006/time#hasBeginning> ;
		rdfs:domain <http://www.w3.org/2006/time#Interval> ;
		rdfs:range  <http://www.w3.org/2006/time#Instant> ;
		rdfs:comment "This property represents the connection between an interval and an instant, used to mark the estimated beginning of a phase."@en ;
		rdfs:label "has estimated beginning"@en .


    ###  http://www.semanticweb.org/albrechtvaatz/ontologies/2025/3/OCP#hasEstimatedEnd
    ocp:hasEstimatedEnd rdf:type owl:ObjectProperty ;
		rdfs:subPropertyOf <http://www.w3.org/2006/time#hasEnd> ;
		rdfs:domain <http://www.w3.org/2006/time#Interval> ;
		rdfs:range  <http://www.w3.org/2006/time#Instant> ;
		rdfs:comment "This property represents the connection between an interval and an instant, used to mark the estimated end of a phase."@en ;
		rdfs:label "has estimated end"@en .


	###  http://www.semanticweb.org/albrechtvaatz/ontologies/2025/3/OCP#isInPhase
    ocp:isInPhase rdf:type owl:ObjectProperty ;
		rdfs:domain ocp:Process ;
		rdfs:range ocp:Phase ;
		rdfs:comment "This property represents the embedding of a process within a phase, used to link a process to the overarching phase it belongs to."@en ;
		rdfs:label "is in phase"@en .


    ###  http://www.semanticweb.org/albrechtvaatz/ontologies/2025/3/OCP#startsCycle
    ocp:startsCycle rdf:type owl:ObjectProperty ;
		rdfs:subPropertyOf <http://www.w3.org/2006/time#hasBeginning> ;
		rdfs:domain <http://www.w3.org/2006/time#Instant> ;
		rdfs:range ocp:Cycle ;
		rdfs:comment "This property represents the relationship between an instant and a cycle, used to mark instants that start a new cycle within a phase."@en ;
		rdfs:label "starts cycle"@en .


    ###  http://www.semanticweb.org/albrechtvaatz/ontologies/2025/3/OCP#startsPhase
    ocp:startsPhase rdf:type owl:ObjectProperty ;
		rdfs:subPropertyOf <http://www.w3.org/2006/time#hasBeginning> ;
		rdfs:domain <http://www.w3.org/2006/time#Instant> ;
		rdfs:range ocp:Phase ;
		rdfs:comment "This property represents the relationship between an instant and a phase, used to mark instants that start a new phase."@en ;
		rdfs:label "starts phase"@en . 


#################################################################
#    Datatype Properties
#################################################################


    ###  http://www.semanticweb.org/albrechtvaatz/ontologies/2025/3/OCP#hasActualTime
    ocp:hasActualTime rdf:type owl:DatatypeProperty ;
		rdfs:subPropertyOf <http://www.w3.org/2006/time#hasTime> ;
		rdfs:domain <http://www.w3.org/2006/time#Instant> ;
		rdfs:range  xsd:date ;
		rdfs:comment "This property represents the connection between an instant and a date, used to mark the actual point in time of an instant."@en ;
		rdfs:label "has actual time"@en .


    ###  http://www.semanticweb.org/albrechtvaatz/ontologies/2025/3/OCP#hasCycleNumber
    ocp:hasCycleNumber rdf:type owl:DatatypeProperty ;
		rdfs:domain ocp:Cycle ;
		rdfs:range xsd:integer ;
		rdfs:comment "This property represents the number of iterations in a cycle, used to specify how many times a process like a planning review repeats."@en ;
		rdfs:label "has cycle number"@en .


    ###  http://www.semanticweb.org/albrechtvaatz/ontologies/2025/3/OCP#hasEstimatedTime
    ocp:hasEstimatedTime rdf:type owl:DatatypeProperty ;
		rdfs:subPropertyOf <http://www.w3.org/2006/time#hasTime> ;
		rdfs:domain <http://www.w3.org/2006/time#Instant> ;
		rdfs:range  xsd:date ;
		rdfs:comment "This property represents the connection between an instant and a date, used to mark the estimated point in time of an instant."@en ;
		rdfs:label "has estimated time"@en .


	###  http://www.semanticweb.org/albrechtvaatz/ontologies/2025/3/OCP#hasProcessID
	ocp:hasProcessID rdf:type owl:DatatypeProperty ;
		rdfs:domain ocp:Process ;
		rdfs:range xsd:string ;
		rdfs:comment "This property represents the unique identifier of a process, used to provide a distinct ID for tracking purposes."@en ;
		rdfs:label "has process ID"@en .


#################################################################
#    Classes
#################################################################

    
    ###  http://www.semanticweb.org/albrechtvaatz/ontologies/2025/3/OCP#Cycle
    ocp:Cycle rdf:type owl:Class ;
		rdfs:subClassOf <http://www.w3.org/2006/time#Interval> ;
		rdfs:comment "This class represents a recurring time span with a starting point, period, and duration, used to track iterating processes."@en ;
		rdfs:label "Cycle"@en .


	###  http://www.semanticweb.org/albrechtvaatz/ontologies/2025/3/OCP#Process		
	ocp:Process rdf:type owl:Class ;
		rdfs:subClassOf <http://www.w3.org/2006/time#Interval> ;
		rdfs:comment "This class represents a complete or partial process as a combination of at least 2 different phases or intervals. Processes can be within phases or intervals."@en ;
		rdfs:label "Process"@en .


    ###  http://www.semanticweb.org/albrechtvaatz/ontologies/2025/3/OCP#Phase
    ocp:Phase rdf:type owl:Class ;
		rdfs:subClassOf <http://www.w3.org/2006/time#Interval> ;
		rdfs:comment "This class represents the main chronological blocks of a building’s process (e.g., planning, construction, usage), serving as a customizable base structure."@en ;
		rdfs:label "Phase"@en .


    ###  http://www.semanticweb.org/albrechtvaatz/ontologies/2025/3/OCP#Transition
    ocp:Transition rdf:type owl:Class ;
		rdfs:subClassOf <http://www.w3.org/2006/time#Instant> ;
		rdfs:comment "This class represents key milestones or triggering events occurring between phases, typically enabling the start of the next phase or marking phase completion."@en ;
		rdfs:label "Transition"@en .


   
